\begin{frame}
    \begin{theorem}[Binomio de Newton]
        Si $a,b\in\mathbb{C}$, entonces
        \begin{math}
            \forall n\in\mathbb{N}\cup\left\{0\right\}:
        \end{math}

        \begin{equation}\label{eq:binomial}
            \left(a+b\right)^{n}=
            \sum\limits_{j=0}^{n}
            \dbinom{n}{j}
            a^{j}
            b^{n-j}.
        \end{equation}
    \end{theorem}

    Derivando~\eqref{eq:binomial} con respecto de $a$, tenemos
    \begin{align}
        \diffp{
            \alert{
                \left(a+b\right)^{n}
            }
        }{a}                    & =
        \diffp{
            \alert{
                \sum\limits_{j=0}^{n}
                \dbinom{n}{j}
                a^{j}
                b^{n-j}
            }
        }{a}.  \notag               \\
        n\left(a+b\right)^{n-1} & =
        \sum\limits_{j=0}^{n}
        \dbinom{n}{j}
        b^{n-j}
        \diffp{
            \alert{
                a^{j}
            }
        }{a}.   \notag              \\
        \alert{a}
        n\left(a+b\right)^{n-1}
                                & =
        \alert{a}
        \sum\limits_{j=0}^{n}
        \dbinom{n}{j}
        \alert{ja^{j-1}}
        b^{n-j}.      \notag        \\
        \label{eq:binomial_I}
        \Aboxed{
            a\left(a+b\right)^{n-1}
                                & =
            \sum\limits_{j=0}^{n}
            \dfrac{j}{n}
            \dbinom{n}{j}
            a^{j}
            b^{n-j}.
        }
    \end{align}
\end{frame}

\begin{frame}
    Derivando~\eqref{eq:binomial} dos veces con respecto de $a$,
    tenemos
    \begin{align}
        \diffp[2]{
            \alert{
                \left(a+b\right)^{n}
            }
        }{a}                   & =
        \diffp[2]{
            \alert{
                \sum\limits_{j=0}^{n}
                \dbinom{n}{j}
                a^{j}
                b^{n-j}
            }
        }{a}.   \notag             \\
        \diffp{
            \alert{
                n\left(a+b\right)^{n-1}
            }
        }{a}                   & =
        \diffp{
            \alert{
                \sum\limits_{j=0}^{n}
                \dbinom{n}{j}
                ja^{j-1}
                b^{n-j}
            }
        }{a}.         \notag       \\
        n\left(n-1\right)
        \left(a+b\right)^{n-2} & =
        \sum\limits_{j=0}^{n}
        \dbinom{n}{j}
        b^{n-j}
        j
        \diffp{
            \alert{
                a^{j-1}
            }
        }{a}.               \notag \\
        \alert{
            \dfrac{a^{2}}{n^{2}}
        }
        n\left(n-1\right)
        \left(a+b\right)^{n-2} & =
        \alert{
            \dfrac{a^{2}}{n^{2}}
        }
        \sum\limits_{j=0}^{n}
        \dbinom{n}{j}
        b^{n-j}
        j
        \alert{
            \left(j-1\right)
            a^{j-2}
        }.                \notag   \\
        \dfrac{n-1}{n}
        a^{2}
        \left(a+b\right)^{n-2}
                               & =
        \sum\limits_{j=0}^{n}
        \dfrac{j\left(j-1\right)}{n^{2}}
        \dbinom{n}{j}
        a^{j}
        b^{n-j}.          \notag   \\
        \label{eq:binomial_II}
        \Aboxed{
            \left(1-\dfrac{1}{n}\right)
            a^{2}
            \left(a+b\right)^{n-2}
                               & =
            \sum\limits_{j=0}^{n}
            \left(
            \dfrac{j^{2}}{n^{2}}-
            \dfrac{j}{n^{2}}
            \right)
            \dbinom{n}{j}
            a^{j}
            b^{n-j}.
        }
    \end{align}
\end{frame}

\begin{frame}
    Definimos
    \begin{math}
        B_{n,j}\left(x\right)\coloneqq
        \dbinom{n}{j}
        x^{j}
            {\left(1-x\right)}^{n-j}
    \end{math}
    para cualquier
    \begin{math}
        \forall j\in\left\{0,\dotsc,n\right\}
    \end{math}.
    Si sustituimos $a=\alert{x}$ y $b=\alert{1-x}$
    en~\eqref{eq:binomial},~\eqref{eq:binomial_I}
    y~\eqref{eq:binomial_II}
    \begin{align}
        \left(\alert{x}+\alert{1-x}\right)^{n} & =
        \sum\limits_{j=0}^{n}
        \dbinom{n}{j}
        \alert{x}^{j}
        {\left(\alert{1-x}\right)}^{n-j}. \notag   \\
        \Aboxed{
        1                                      & =
            \sum\limits_{j=0}^{n}
            B_{n,j}\left(x\right).
        }                                          \\
        \alert{x}\left(\alert{x}+\alert{1-x}\right)^{n-1}
                                               & =
        \sum\limits_{j=0}^{n}
        \dfrac{j}{n}
        \dbinom{n}{j}
        \alert{x}^{j}
        {\left(\alert{1-x}\right)}^{n-j}. \notag   \\
        \Aboxed{
            x
                                               & =
            \sum\limits_{j=0}^{n}
            \dfrac{j}{n}
            B_{n,j}\left(x\right).
        }                                          \\
        \left(1-\dfrac{1}{n}\right)
        \alert{x}^{2}
        \left(\alert{x}+\alert{1-x}\right)^{n-2}
                                               & =
        \sum\limits_{j=0}^{n}
        \left(
        \dfrac{j^{2}}{n^{2}}-
        \dfrac{j}{n^{2}}
        \right)
        \dbinom{n}{j}
        \alert{x}^{j}
        {\left(\alert{1-x}\right)}^{n-j}.
        \notag                                     \\
        \left(1-\dfrac{1}{n}\right)
        x^{2}
                                               & =
        \sum\limits_{j=0}^{n}
        \left(
        \dfrac{j^{2}}{n^{2}}-
        \dfrac{j}{n^{2}}
        \right)
        B_{n,j}\left(x\right)=
        \sum\limits_{j=0}^{n}
        \dfrac{j^{2}}{n^{2}}
        B_{n,j}\left(x\right)-
        \dfrac{1}{n}
        \alert{
            \sum\limits_{j=0}^{n}
            \dfrac{j}{n}
            B_{n,j}\left(x\right)
        }.
        \notag                                     \\
        \Aboxed{
            \left(1-\dfrac{1}{n}\right)
            x^{2}+
            \dfrac{\alert{x}}{n}
                                               & =
            \sum\limits_{j=0}^{n}
            \dfrac{j^{2}}{n^{2}}
            B_{n,j}\left(x\right).
        }
    \end{align}
\end{frame}