\section{Pregunta N$^{\circ}$6\qquad Le√≥n Alonzo Terrones Caccha}

\input{interpolation}
% \input{interpolation_theorems}

\begin{frame}
	\begin{enumerate}\setcounter{enumi}{5}
		\item

		      Encuentre el interpolante de Lagrange
		      \begin{math}
			      p_{2}\left(t\right)=
			      \sum\limits_{k=0}^{2}
			      x_{k}
			      \ell_{k}\left(t\right)
		      \end{math}
		      para el conjunto de datos
		      \begin{math}
			      \left\{
			      \left(0,1\right),
			      \left(\frac{1}{2},2\right),
			      \left((1,\frac{3}{2}\right),
                    \left((2,-1\right)
			      \right\}
		      \end{math}.
		      Encuentre $p_{2,k}$ en
		      \begin{math}
			      p_{2}\left(t\right)=
			      \sum\limits_{k=0}^{2}
			      p_{2,k}t^{k}
		      \end{math}.
	\end{enumerate}

	\begin{solution}
		\begin{align*}
			\ell_{0}\left(t\right) & =
			\prod\limits_{\substack{j=0        \\j\neq 0}}^{n}
			\dfrac{t-t_{j}}{t_{0}-t_{j}}=
			\dfrac{\left(t-t_{1}\right)\left(t-t_{2}\right)}{\left(t_{0}-t_{1}\right)\left(t_{0}-t_{2}\right)}=
			\dfrac{\left(t-0\right)\left(t-1\right)}{\left(\left(-1\right)-0\right)\left(\left(-1\right)-1\right)}=
			\dfrac{1}{2}t\left(t-1\right).     \\
			\ell_{1}\left(t\right) & =
			\prod\limits_{\substack{j=0        \\j\neq 1}}^{n}
			\dfrac{t-t_{j}}{t_{1}-t_{j}}=
			\dfrac{\left(t-t_{0}\right)\left(t-t_{2}\right)}{\left(t_{1}-t_{0}\right)\left(t_{1}-t_{2}\right)}=
			\dfrac{\left(t-\left(-1\right)\right)\left(t-1\right)}{\left(0-\left(-1\right)\right)\left(0-1\right)}=
			-\left(t+1\right)\left(t-1\right). \\
			\ell_{2}\left(t\right) & =
			\prod\limits_{\substack{j=0        \\j\neq 2}}^{n}
			\dfrac{t-t_{j}}{t_{2}-t_{j}}=
			\dfrac{\left(t-t_{0}\right)\left(t-t_{1}\right)}{\left(t_{2}-t_{0}\right)\left(t_{2}-t_{1}\right)}=
			\dfrac{\left(t-\left(-1\right)\right)\left(t-0\right)}{\left(1-\left(-1\right)\right)\left(1-0\right)}=
			\dfrac{1}{2}\left(t+1\right)t.
		\end{align*}

		Entonces,
		\begin{align*}
			p_{2}\left(t\right) & =
			\sum\limits_{k=0}^{2}
			x_{k}
			\ell_{k}\left(t\right)=
			\alert{x_{0}}\ell_{0}\left(t\right)+
			\alert{x_{1}}\ell_{1}\left(t\right)+
			\alert{x_{2}}\ell_{2}\left(t\right)=
			\dfrac{1}{2}\ell_{0}\left(t\right)+
			\ell_{1}\left(t\right)-
			\ell_{2}\left(t\right).               \\
			                    & =
			\dfrac{1}{2}\alert{\dfrac{1}{2}t\left(t-1\right)}
			\alert{-\left(t+1\right)\left(t-1\right)}-
			\alert{\dfrac{1}{2}\left(t+1\right)t}. \\
			                    & =
			-1.25t^{2}-0.75t+1.
		\end{align*}
	\end{solution}
\end{frame}

\begin{frame}
	\begin{solution}
		\begin{figure}[ht!]
			\centering
			\includegraphics[width=.8\paperwidth]{p6_lagrange}
		\end{figure}
	\end{solution}
\end{frame}


\begin{frame}
	\begin{solution}
		\begin{figure}[ht!]
			\centering
			\includegraphics[width=.8\paperwidth]{p6}
		\end{figure}
	\end{solution}
\end{frame}