\section{Pregunta N$^{\circ}$9\qquad Carlos Alonso Aznarán Laos}

\begin{frame}
    \begin{enumerate}\setcounter{enumi}{8}
        \item

              Encuentre una expresión general para
              \begin{math}
                  \ell_{k}^{\left(1\right)}\left(t\right)=
                  \diff{\ell_{k}\left(t\right)}{t}
              \end{math}.
    \end{enumerate}

    \begin{solution}
        Si
        \begin{math}
            \ell_{k}
            \left(t\right)
            \overset{\text{def}}{=}
            \prod\limits_{\substack{j=0\\j\neq k}}^{n}
            \dfrac{t-t_{j}}{t_{k}-t_{j}}
        \end{math}, entonces
        \begin{math}
            \alert{\ln}
            \left(
            \ell_{k}
            \left(t\right)
            \right)=
            \alert{\ln}
            \left(
            \prod\limits_{\substack{j=0\\j\neq k}}^{n}
            \dfrac{t-t_{j}}{t_{k}-t_{j}}
            \right)=
            \sum\limits_{\substack{j=0\\j\neq k}}^{n}
            \ln
            \left(
            \dfrac{t-t_{j}}{t_{k}-t_{j}}
            \right)=
            \sum\limits_{\substack{j=0\\j\neq k}}^{n}
            \ln
            \left(
            t-t_{j}
            \right)-
            \sum\limits_{\substack{j=0\\j\neq k}}^{n}
            \left(
            t_{k}-t_{j}
            \right)
        \end{math}.
        Derivando,

        \begin{align*}
            {\left(
                \ln
                \left(
                    \ell_{k}
                    \left(t\right)
                    \right)
            \right)}^{\prime} & =
            {\left(
            \sum\limits_{\substack{j=0  \\j\neq k}}^{n}
            \ln
            \left(
            t-t_{j}
            \right)
            -\sum\limits_{\substack{j=0 \\j\neq k}}^{n}
            \left(
            t_{k}-t_{j}
            \right)
            \right)}^{\prime}=
            \sum\limits_{\substack{j=0  \\j\neq k}}^{n}
            {\left(
                \ln
                \left(
                t-t_{j}
                \right)
                \right)}^{\prime}.
            \\
            \dfrac{
                \ell^{\prime}_{k}
                \left(t\right)
            }{
                \alert{
                    \ell_{k}
                    \left(t\right)
                }
            }                 & =
            \sum\limits_{\substack{j=0  \\j\neq k}}^{n}
            \dfrac{{\left(t-t_{j}\right)}^{\prime}}{t-t_{j}}=
            \sum\limits_{\substack{j=0  \\j\neq k}}^{n}
            \dfrac{1}{t-t_{j}}.
            \\
            \Aboxed{
            \ell^{\prime}_{k}
            \left(t\right)    & =
            \alert{
                \ell_{k}
                \left(t\right)
            }
            \sum\limits_{\substack{j=0  \\j\neq k}}^{n}
            \dfrac{1}{t-t_{j}}.
            }
        \end{align*}
    \end{solution}
\end{frame}